Updates to vale.dfy and machine.dfy (WIP)

arch/riscv/machine.s.dfy
@@ -81,13 +81,99 @@ module rv_machine {
         }
     }
 
-    // datatype uint64_raw = uint64_cons(
-    //     lh: uint32, uh: uint32, full: uint64)
+    // base integer instruction set, 32-bit
+    datatype ins32 =
+    | RV_LB(rd: reg32_t, rs1: reg32_t, oimm12: uint32)
+    | RV_LH (rd: reg32_t, rs1: reg32_t, oimm12: uint32)
+    | RV_LW (rd: reg32_t, rs1: reg32_t, oimm12: uint32)
+    | RV_LBU (rd: reg32_t, rs1: reg32_t, oimm12: uint32)
+    | RV_LHU (rd: reg32_t, rs1: reg32_t, oimm12: uint32)
 
-    // type uint64_view_t = num: uint64_raw |
-    //     && num.lh == dw_lh(num.full)
-    //     && num.uh == dw_uh(num.full)
-    //     witness *
+    | RV_FENCE (pred: uint32, succ: uint32)
+    | RV_FENCE_I
+
+    | RV_ADDI (rd: reg32_t, rs1: reg32_t, simm12: int32) // sign extends, ignore overflow
+    | RV_SLLI (rd: reg32_t, rs1: reg32_t, shamt6: uint32) // logical left shift
+    | RV_SLTI (rd: reg32_t, rs1: reg32_t, simm12: int32) // sign extend, 1 if rs1 (signed) < imm, else 0
+    | RV_SLTIU (rd: reg32_t, rs1: reg32_t, imm12: uint32) // compare both vals as unsigned.
+    | RV_XORI (rd: reg32_t, rs1: reg32_t, imm12: uint32)
+    | RV_ORI (rd: reg32_t, rs1: reg32_t, imm12: uint32)
+    | RV_ANDI (rd: reg32_t, rs1: reg32_t, imm12: uint32)
+    | RV_SRLI (rd: reg32_t, rs1: reg32_t, shamt6: uint32) // logical right shift
+    | RV_SRAI (rd: reg32_t, rs1: reg32_t, shamt6: uint32) // arithmetic right shift
+
+    | RV_AUIPC (rd: reg32_t, oimm20: uint32)
+
+    | RV_SB (rs1: reg32_t, rs2: reg32_t, imm12: uint32)
+    | RV_SH (rs1: reg32_t, rs2: reg32_t, imm12: uint32)
+    | RV_SW (rs1: reg32_t, rs2: reg32_t, imm12: uint32)
+
+    | RV_ADD (rd: reg32_t, rs1: reg32_t, rs2: reg32_t) // ignore overflow
+    | RV_SUB (rd: reg32_t, rs1: reg32_t, rs2: reg32_t) // ignore overflow
+    | RV_SLL (rd: reg32_t, rs1: reg32_t, rs2: reg32_t) // shift logical left by "lower 5 bits of rs2"
+    | RV_SLT (rd: reg32_t, rs1: reg32_t, rs2: reg32_t) // signed less than
+    | RV_SLTU (rd: reg32_t, rs1: reg32_t, rs2: reg32_t) // unsigned less than
+    | RV_XOR (rd: reg32_t, rs1: reg32_t, rs2: reg32_t) // bitwise
+    | RV_SRL (rd: reg32_t, rs1: reg32_t, rs2: reg32_t) // shift logical right by "lower 5 bits of rs2"
+    | RV_SRA (rd: reg32_t, rs1: reg32_t, rs2: reg32_t) // shift arithmetic right by "lower 5 bits of rs2"
+    | RV_OR (rd: reg32_t, rs1: reg32_t, rs2: reg32_t) // bitwise
+    | RV_AND (rd: reg32_t, rs1: reg32_t, rs2: reg32_t) // bitwise
+
+    | RV_LUI (rd: reg32_t, imm20: uint32)
+    | RV_LI (rd: reg32_t, imm20: uint32)
+
+    // | RV_BEQ (rs1: reg32_t, rs2: reg32_t, sbimm12: uint32)
+    // | RV_BNE (rs1: reg32_t, rs2: reg32_t, sbimm12: uint32)
+    // | RV_BLT (rs1: reg32_t, rs2: reg32_t, sbimm12: uint32)
+    // | RV_BGE (rs1: reg32_t, rs2: reg32_t, sbimm12: uint32)
+    // | RV_BLTU (rs1: reg32_t, rs2: reg32_t, sbimm12: uint32)
+    // | RV_BGEU (rs1: reg32_t, rs2: reg32_t, sbimm12: uint32)
+    // 
+    // | RV_JALR (rd: reg32_t, rs1: reg32_t, oimm12: uint32)
+    // | RV_JAL (rd: reg32_t, jimm20: uint32)
+
+    // standard extension for integer mult and div, 32-bit
+    | RV_MUL (rd: reg32_t, rs1: reg32_t, rs2: reg32_t)
+    | RV_MULH (rd: reg32_t, rs1: reg32_t, rs2: reg32_t)
+    | RV_MULHSU (rd: reg32_t, rs1: reg32_t, rs2: reg32_t)
+    | RV_MULHU (rd: reg32_t, rs1: reg32_t, rs2: reg32_t)
+    | RV_DIV (rd: reg32_t, rs1: reg32_t, rs2: reg32_t)
+    | RV_DIVU (rd: reg32_t, rs1: reg32_t, rs2: reg32_t)
+    | RV_REM (rd: reg32_t, rs1: reg32_t, rs2: reg32_t)
+    | RV_REMU (rd: reg32_t, rs1: reg32_t, rs2: reg32_t)
+
+    // control and status register extension
+    | RISC_ECALL
+    | RISC_EBREAK
+    | RISC_URET
+    | RISC_SRET
+    | RISC_MRET
+    | RISC_WFI
+    | RISC_SFENCE_VMA (rs1: reg32_t, rs2: reg32_t)
+    | RISC_CSRRW (rd: reg32_t, rs1: reg32_t, csr12: uint32)
+    | RISC_CSRRS (rd: reg32_t, rs1: reg32_t, csr12: uint32)
+    | RISC_CSRRC (rd: reg32_t, rs1: reg32_t, csr12: uint32)
+    | RISC_CSRRWI (rd: reg32_t, zimm: uint32, csr12: uint32)
+    | RISC_CSRRSI (rd: reg32_t, zimm: uint32, csr12: uint32)
+    | RISC_CSRRCI (rd: reg32_t, zimm: uint32, csr12: uint32)
+
+    /* control flow definitions */
+
+    datatype cmp = Eq | Ne | Le | Ge | Lt | Gt
+    
+    datatype cond = Cmp(op:cmp, r1:reg32_t, r2:reg32_t)
+
+    datatype code =
+    | Ins32(ins: ins32)
+    | Block(block: codes)
+    | While(whileCond: cond, whileBody: code)
+    | IfElse(ifCond: cond, ifTrue: code, ifFalse: code)
+    | Function(name: string, functionBody: codes)
+    | Comment(com: string)
+
+    datatype codes =
+      | CNil
+      | va_CCons(hd: code, tl: codes)
 
    /* memory definitions */ 
 
@@ -178,170 +264,83 @@ module rv_machine {
         {
             this.(regs := this.regs[reg32_to_index(r) := value])
         }
+
+        function method eval_ins32(ins: ins32): state
+        {
+            if !ok then
+                this
+            else match ins
+              case _ => this // TODO: executable semantics
+        }
+
+        function method eval_block(block: codes): state
+            decreases block
+        {
+            if block.CNil? then
+                this
+            else
+                eval_code(block.hd).eval_block(block.tl)
+        }
+
+        function eval_cond(c:cond): bool
+        {
+            eval_cmp(c)
+        }
+
+        function method eval_while(condition: cond, body: code, n: nat): state
+            decreases body, n
+        {
+            if !ok then
+                this
+            else
+              exists n:nat :: eval_while(condition, body, n)
+              
+                if n == 0 then
+                    this
+                else
+                  eval_code(body).eval_while(condition, body, n - 1)
+        }
+
+        function method eval_cmp(cond: cond): bool
+        {
+            var Cmp(op, r1, r2) := cond;
+            match op 
+                case Eq => (read_reg32(r1) == read_reg32(r2))
+                case Ne => (read_reg32(r1) != read_reg32(r2))
+                case Le => (read_reg32(r1) <= read_reg32(r2))
+                case Lt => (read_reg32(r1) < read_reg32(r2))
+                case Gt => (read_reg32(r1) > read_reg32(r2))
+                case Ge => (read_reg32(r1) >= read_reg32(r2))
+        }
+
+        function method eval_if_else(cond: cond, ifT: code, ifF: code): state
+            decreases if eval_cmp(cond) then ifT else ifF
+        {
+            if !ok then
+                this
+            else
+                if eval_cmp(cond) then
+                    eval_code(ifT)
+                else
+                    eval_code(ifF)
+        }
+
+        function method eval_code(c: code): state
+            decreases c, 0
+        {
+            match c
+                case Ins32(ins) => eval_ins32(ins)
+                case Block(block) => eval_block(block)
+                case IfElse(cond, ifT, ifF) => eval_if_else(cond, ifT, ifF)
+                case While(cond, body) => eval_while(cond, body)
+                case Function(name, body) => eval_block(body)
+                case Comment(com) => this
+        }
     }
 
     predicate valid_state(s: state)
     {
         s.ok
     }
-    
-    // base integer instruction set, 32-bit
-    datatype ins32 =
-    | RV_LB(rd: reg32_t, rs1: reg32_t, oimm12: uint32)
-    | RV_LH (rd: reg32_t, rs1: reg32_t, oimm12: uint32)
-    | RV_LW (rd: reg32_t, rs1: reg32_t, oimm12: uint32)
-    | RV_LBU (rd: reg32_t, rs1: reg32_t, oimm12: uint32)
-    | RV_LHU (rd: reg32_t, rs1: reg32_t, oimm12: uint32)
 
-    | RV_FENCE (pred: uint32, succ: uint32)
-    | RV_FENCE_I
-
-    | RV_ADDI (rd: reg32_t, rs1: reg32_t, simm12: int32) // sign extends, ignore overflow
-    | RV_SLLI (rd: reg32_t, rs1: reg32_t, shamt6: uint32) // logical left shift
-    | RV_SLTI (rd: reg32_t, rs1: reg32_t, simm12: int32) // sign extend, 1 if rs1 (signed) < imm, else 0
-    | RV_SLTIU (rd: reg32_t, rs1: reg32_t, imm12: uint32) // compare both vals as unsigned.
-    | RV_XORI (rd: reg32_t, rs1: reg32_t, imm12: uint32)
-    | RV_ORI (rd: reg32_t, rs1: reg32_t, imm12: uint32)
-    | RV_ANDI (rd: reg32_t, rs1: reg32_t, imm12: uint32)
-    | RV_SRLI (rd: reg32_t, rs1: reg32_t, shamt6: uint32) // logical right shift
-    | RV_SRAI (rd: reg32_t, rs1: reg32_t, shamt6: uint32) // arithmetic right shift
-
-    | RV_AUIPC (rd: reg32_t, oimm20: uint32)
-
-    | RV_SB (rs1: reg32_t, rs2: reg32_t, imm12: uint32)
-    | RV_SH (rs1: reg32_t, rs2: reg32_t, imm12: uint32)
-    | RV_SW (rs1: reg32_t, rs2: reg32_t, imm12: uint32)
-
-    | RV_ADD (rd: reg32_t, rs1: reg32_t, rs2: reg32_t) // ignore overflow
-    | RV_SUB (rd: reg32_t, rs1: reg32_t, rs2: reg32_t) // ignore overflow
-    | RV_SLL (rd: reg32_t, rs1: reg32_t, rs2: reg32_t) // shift logical left by "lower 5 bits of rs2"
-    | RV_SLT (rd: reg32_t, rs1: reg32_t, rs2: reg32_t) // signed less than
-    | RV_SLTU (rd: reg32_t, rs1: reg32_t, rs2: reg32_t) // unsigned less than
-    | RV_XOR (rd: reg32_t, rs1: reg32_t, rs2: reg32_t) // bitwise
-    | RV_SRL (rd: reg32_t, rs1: reg32_t, rs2: reg32_t) // shift logical right by "lower 5 bits of rs2"
-    | RV_SRA (rd: reg32_t, rs1: reg32_t, rs2: reg32_t) // shift arithmetic right by "lower 5 bits of rs2"
-    | RV_OR (rd: reg32_t, rs1: reg32_t, rs2: reg32_t) // bitwise
-    | RV_AND (rd: reg32_t, rs1: reg32_t, rs2: reg32_t) // bitwise
-
-    | RV_LUI (rd: reg32_t, imm20: uint32)
-    | RV_LI (rd: reg32_t, imm20: uint32)
-
-    // | RV_BEQ (rs1: reg32_t, rs2: reg32_t, sbimm12: uint32)
-    // | RV_BNE (rs1: reg32_t, rs2: reg32_t, sbimm12: uint32)
-    // | RV_BLT (rs1: reg32_t, rs2: reg32_t, sbimm12: uint32)
-    // | RV_BGE (rs1: reg32_t, rs2: reg32_t, sbimm12: uint32)
-    // | RV_BLTU (rs1: reg32_t, rs2: reg32_t, sbimm12: uint32)
-    // | RV_BGEU (rs1: reg32_t, rs2: reg32_t, sbimm12: uint32)
-    // 
-    // | RV_JALR (rd: reg32_t, rs1: reg32_t, oimm12: uint32)
-    // | RV_JAL (rd: reg32_t, jimm20: uint32)
-
-    // standard extension for integer mult and div, 32-bit
-    | RV_MUL (rd: reg32_t, rs1: reg32_t, rs2: reg32_t)
-    | RV_MULH (rd: reg32_t, rs1: reg32_t, rs2: reg32_t)
-    | RV_MULHSU (rd: reg32_t, rs1: reg32_t, rs2: reg32_t)
-    | RV_MULHU (rd: reg32_t, rs1: reg32_t, rs2: reg32_t)
-    | RV_DIV (rd: reg32_t, rs1: reg32_t, rs2: reg32_t)
-    | RV_DIVU (rd: reg32_t, rs1: reg32_t, rs2: reg32_t)
-    | RV_REM (rd: reg32_t, rs1: reg32_t, rs2: reg32_t)
-    | RV_REMU (rd: reg32_t, rs1: reg32_t, rs2: reg32_t)
-
-    // control and status register extension
-    | RISC_ECALL
-    | RISC_EBREAK
-    | RISC_URET
-    | RISC_SRET
-    | RISC_MRET
-    | RISC_WFI
-    | RISC_SFENCE_VMA (rs1: reg32_t, rs2: reg32_t)
-    | RISC_CSRRW (rd: reg32_t, rs1: reg32_t, csr12: uint32)
-    | RISC_CSRRS (rd: reg32_t, rs1: reg32_t, csr12: uint32)
-    | RISC_CSRRC (rd: reg32_t, rs1: reg32_t, csr12: uint32)
-    | RISC_CSRRWI (rd: reg32_t, zimm: uint32, csr12: uint32)
-    | RISC_CSRRSI (rd: reg32_t, zimm: uint32, csr12: uint32)
-    | RISC_CSRRCI (rd: reg32_t, zimm: uint32, csr12: uint32)
-
-    predicate eval_ins32(ins: ins32, s: state, r: state)
-    {
-        if !s.ok then
-            !r.ok
-        else
-            r.ok && (valid_state(s) ==> valid_state(r))
-    }
-
-    /* control flow definitions */
-
-    datatype cmp = Eq | Ne | Le | Ge | Lt | Gt
-    
-    datatype cond = Cmp(op:cmp, r1:reg32_t, r2:reg32_t)
-
-    datatype code =
-    | Ins32(ins: ins32)
-    | Block(block: codes)
-    | While(whileCond: cond, whileBody: code)
-    | IfElse(ifCond: cond, ifTrue: code, ifFalse: code)
-    | Function(name: string, functionBody: codes)
-    | Comment(com: string)
-
-    datatype codes =
-      | CNil
-      | va_CCons(hd: code, tl: codes)
-
-    predicate eval_block(block: codes, s: state, r: state)
-    {
-        if block.CNil? then
-            r == s
-        else
-            exists r': state :: eval_code(block.hd, s, r') && eval_block(block.tl, r', r)
-    }
-
-    function eval_cmp(s:state, c:cmp, r1:reg32_t, r2:reg32_t):bool
-    {
-        match c
-          case Eq  => s.read_reg32(r1) == s.read_reg32(r2)
-          case Ne => s.read_reg32(r1) != s.read_reg32(r2)
-          case Le  => s.read_reg32(r1) <= s.read_reg32(r2)
-          case Ge  => s.read_reg32(r1) >= s.read_reg32(r2)
-          case Lt  => s.read_reg32(r1) < s.read_reg32(r2)
-          case Gt  => s.read_reg32(r1) > s.read_reg32(r2)
-    }
-
-    function eval_cond(s:state, c:cond):bool
-    {
-        eval_cmp(s, c.op, c.r1, c.r2)
-    }
-
-    predicate eval_if_else(cond:cond, ifT:code, ifF:code, s:state, r:state)
-        decreases if eval_cond(s, cond) then ifT else ifF
-    {
-        if s.ok then
-            (if eval_cond(s, cond) then eval_code(ifT, s, r) else eval_code(ifF, s, r))
-        else
-            !r.ok
-    }
-
-    predicate eval_while(condition:cond, body:code, n: nat, s: state, r: state)
-        decreases body, n
-    {
-        if s.ok then
-            if n == 0 then
-                !eval_cond(s, condition) && (s == r)
-            else
-              exists s': state :: eval_cond(s, condition)
-                      && eval_code(body, s, s')
-                      && eval_while(condition, body, n - 1, s', r)
-        else
-            !r.ok
-    }
-
-    predicate eval_code(c: code, s: state, r: state)
-        decreases c, 0
-    {
-        match c
-            case Ins32(ins) => eval_ins32(ins, s, r)
-            case Block(block) => eval_block(block, s, r)
-            case While(condition, body) => exists n:nat :: eval_while(condition, body, n, s, r)
-            case IfElse(cond, ifT, ifF) => eval_if_else(cond, ifT, ifF, s, r)
-            case Comment(com) => s == r
-    }
 }
