arch/riscv/vale.i.dfy
@@ -1,14 +1,18 @@
 include "machine.s.dfy"
+include "../../std_lib/src/NonlinearArithmetic/Mul.dfy"
 
 module rv_vale {
     import opened integers
     import opened rv_machine
 
-    type va_code = code
-    type va_codes = codes
-    type va_state = state
+    import bv32_ops
+    import bv32_seq
+    import Mul
+
+    //  pair/seq
 
     function fst<T,Q>(t:(T, Q)) : T { t.0 }
+
     function snd<T,Q>(t:(T, Q)) : Q { t.1 }
 
     function seq_len<T>(s: seq<T>): nat
@@ -26,34 +30,98 @@ module rv_vale {
         xs + [x]
     }
 
+    function ToNat(xs: seq<uint32>): nat
+    {
+        bv32_seq.ToNatRight(xs)
+    }
+
+    function SeqZero(n: nat): seq<uint32>
+    {
+        bv32_seq.SeqZero(n)
+    }
+
     function mod(a: int, n: nat): int
         requires n != 0;
     {
         a % n
     }
 
-    function mod_add(a: nat, b: nat, m: nat): nat 
-        requires a < m && b < m;
+    // need this for mul
+
+    function va_mul_nat(a: nat, b: nat): nat
     {
-        if a + b > m then a + b - m else a + b
+        Mul.LemmaMulNonnegativeAuto();
+        a * b
     }
 
-    function va_get_ok(s: va_state): bool
+    function method uint32_addi(x: uint32, y: bv32_ops.sint): uint32
     {
-        s.ok
+        bv32_ops.addi(x, y)
     }
 
-    function va_get_reg32_t(r : reg32_t, s: va_state): uint32
+    function method uint32_add(x: uint32, y: uint32): uint32
+    {
+        bv32_ops.add(x, y)
+    }
+
+    function method uint32_andi(x: uint32, y: bv32_ops.sint): uint32
+    {
+        bv32_ops.andi(x, y)
+    }
+
+    // otbn state realted
+
+    type va_code = code
+
+    type va_codes = codes
+
+    type va_state = state
+
+    // reg32
+
+    type va_value_reg32 = uint32
+
+    type va_operand_reg32 = reg32_t
+
+    function va_get_reg32_t(r: reg32_t, s: va_state): uint32
     {
         s.read_reg32(r)
     }
 
-    function va_eval_reg32(s: va_state, r : reg32_t): uint32
+    function va_update_reg32_t(r: reg32_t, sM: va_state, sK: va_state): va_state
     {
-        s.read_reg32(r)
+        var index := reg32_to_index(r);
+        sK.(regs := sK.regs[index := sM.regs[index]])
     }
 
-    function va_get_mem(s: va_state): mem_t
+    predicate va_is_src_reg32(r: reg32_t, s: va_state)
+    {
+        true
+    }
+
+    predicate va_is_dst_reg32(r: reg32_t, s: va_state)
+    {
+        r.index != 0 && r.index != 1
+    }
+
+    function va_eval_reg32(s: va_state, r: reg32_t):uint32
+    {
+        va_get_reg32_t(r, s)
+    }
+
+    function va_update_operand_reg32(r: reg32_t, sM: va_state, sK: va_state): va_state
+    {
+        va_update_reg32_t(r, sM, sK)
+    }
+
+    function method va_op_cmp_reg32_t(r: reg32_t) : reg32_t
+    {
+        r
+    }
+
+    // mem
+
+    function va_get_mem(s: va_state): map<int, uint32>
     {
         s.mem
     }
@@ -63,62 +131,16 @@ module rv_vale {
         sK.(mem := sM.mem)
     }
 
+    // ok
+
     function va_update_ok(sM: va_state, sK: va_state): va_state
     {
         sK.(ok := sM.ok)
     }
 
-    function va_update_reg32_t(r: reg32_t, sM: va_state, sK: va_state): va_state
+    function va_get_ok(s: va_state): bool
     {
-        var index := reg32_to_index(r);
-        sK.(regs := sK.regs[index := sM.regs[index]])
-    }
-
-    type va_operand_simm32 = int32
-    predicate va_is_src_simm32(v:int32, s: va_state) { true }
-    function va_eval_simm32(s: va_state, v:int32):int32 { v }
-    function method va_const_simm32(n:int32):int32 { n }
-
-    type va_operand_imm32 = uint32
-    predicate va_is_src_imm32(v:uint32, s: va_state) { true }
-    function va_eval_imm32(s: va_state, v:uint32):uint32 { v }
-    function method va_const_imm32(n:uint32):uint32 { n }
-
-    function va_mul_nat(a: nat, b: nat): nat
-    {
-        //assume false;
-        a * b
-    }
-
-    // reg32
-
-    type va_value_reg32 = uint32
-
-    type va_operand_reg32 = reg32_t
-
-    predicate va_is_src_reg32(r: reg32_t, s: va_state)
-    {
-        true
-    }
-
-    predicate va_is_dst_reg32(r: reg32_t, s: va_state)
-    {
-        !r.X0?
-    }
-
-    function va_read_reg32(s: va_state, r : reg32_t):uint32
-    {
-        s.read_reg32(r)
-    }
-
-    function va_update_operand_reg32(r: reg32_t, sM: va_state, sK: va_state): va_state
-    {
-        va_update_reg32_t(r, sM, sK)
-    }
-
-    function method va_op_cmp_reg32_t(r : reg32_t)  : reg32_t
-    {
-        r
+        s.ok
     }
 
     predicate va_state_eq(s0: va_state, s1: va_state)
@@ -129,34 +151,49 @@ module rv_vale {
         && s0.ok == s1.ok
     }
 
-    predicate{:opaque} eval_code_opaque(c:code, s0:state, sN:state)
+    // control flow lemmas
+
+    predicate{:opaque} eval_code_opaque(c: code, s0: state, sN: state)
     {
-        eval_code(c, s0, sN)
+        sN == s0.eval_code(c)
     }
 
-    predicate eval_code_lax(c:code, s:state, r:state)
+    predicate eval_code_lax(c: code, s: va_state, r: va_state)
     {
         s.ok ==> eval_code_opaque(c, s, r)
     }
 
-    function method va_CNil():codes { CNil }
-    predicate cHeadIs(b:codes, c:code) { b.va_CCons? && b.hd == c }
-    predicate cTailIs(b:codes, t:codes) { b.va_CCons? && b.tl == t }
-
-    predicate va_require(b0:codes, c1:code, s0: va_state, sN: va_state)
+    predicate {:opaque} valid_state_opaque(s: va_state)
+        ensures valid_state_opaque(s) ==> valid_state(s);
     {
-        && cHeadIs(b0, c1)
-        && eval_code_lax(Block(b0), s0, sN)
+        && s.ok
+        && valid_state(s)
+    }
+
+    function method va_CNil(): codes { CNil }
+
+    predicate cHeadIs(b: codes, c: code) { b.va_CCons? && b.hd == c }
+
+    predicate cTailIs(b: codes, t: codes) { b.va_CCons? && b.tl == t }
+
+    predicate va_require(
+        complete_block: codes,
+        head_code: code,
+        s0: va_state,
+        sN: va_state)
+    {
+        && cHeadIs(complete_block, head_code)
+        && eval_code_lax(Block(complete_block), s0, sN)
         && valid_state_opaque(s0)
     }
 
     // Weaker form of eval_code that we can actually ensure generically in instructions
-    predicate eval_weak(c:code, s:state, r:state)
+    predicate eval_weak(c: code, s: va_state, r: va_state)
     {
         s.ok && r.ok ==> eval_code_opaque(c, s, r)
     }
 
-    predicate va_ensure(b0:codes, b1:codes, s0: va_state, s1: va_state, sN: va_state)
+    predicate va_ensure(b0: codes, b1: codes, s0: va_state, s1: va_state, sN: va_state)
     {
         && cTailIs(b0, b1)
         && eval_weak(b0.hd, s0, s1)
@@ -168,7 +205,7 @@ module rv_vale {
     {
     }
 
-    function method va_const_cmp(n:uint32):uint32 { n }
+    function method va_const_cmp(n: uint32):uint32 { n }
     function method va_coerce_reg32_to_cmp(r: reg32_t): reg32_t { r }
 
     function method va_cmp_eq(r1:reg32_t, r2:reg32_t):cond { Cmp(Eq, r1, r2) }
@@ -179,33 +216,35 @@ module rv_vale {
     function method va_cmp_gt(r1:reg32_t, r2:reg32_t):cond { Cmp(Gt, r1, r2) }
 
     function method va_op_reg32_reg32_t(r: reg32_t): reg32_t { r }
-    function method va_Block(block:codes):code { Block(block) }
-    function method va_While(wcond:cond, wcode:code):code { While(wcond, wcode) }
+
+    function method va_Block(block:codes): code { Block(block) }
+    function method va_While(wcond: cond, wcode: code): code { While(wcond, wcode) }
     function method va_Function(name: string, body: codes): code { Function(name, body) }
-    function method va_IfElse(ifb:cond, ift:code, iff:code):code { IfElse(ifb, ift, iff) }
+    function method va_IfElse(ifb: cond, ift:code, iff:code):code { IfElse(ifb, ift, iff) }
 
     function method va_get_block(c: code): codes requires c.Block? || c.Function? { 
         if c.Block? then c.block else c.functionBody }
-    function method va_get_whileCond(c:code):cond requires c.While? {c.whileCond }
-    function method va_get_whileBody(c:code):code requires c.While? { c.whileBody }
+    function method va_get_whileCond(c: code): cond requires c.While? {c.whileCond }
+    function method va_get_whileBody(c: code): code requires c.While? { c.whileBody }
     function method va_get_ifCond(c:code):cond requires c.IfElse? { c.ifCond }
     function method va_get_ifTrue(c:code):code requires c.IfElse? { c.ifTrue }
     function method va_get_ifFalse(c:code):code requires c.IfElse? { c.ifFalse }
 
-    lemma lemma_FailurePreservedByBlock(block:codes, s:state, r:state)
-        requires eval_block(block, s, r);
+
+    lemma lemma_FailurePreservedByBlock(block: codes, s: state, r: state)
+        requires r == s.eval_block(block);
         ensures !s.ok ==> !r.ok;
         decreases block;
     {
         if !block.CNil? {
-            var r' :| eval_code(block.hd, s, r') && eval_block(block.tl, r', r);
+            var r' :| r' == s.eval_code(block.hd) && r == r'.eval_block(block.tl);
             lemma_FailurePreservedByCode(block.hd, s, r');
             lemma_FailurePreservedByBlock(block.tl, r', r);
         }
     }
 
-    lemma lemma_FailurePreservedByCode(c:code, s:state, r:state)
-        requires eval_code(c, s, r);
+    lemma lemma_FailurePreservedByCode(c: code, s: state, r: state)
+        requires r == s.eval_code(c);
         ensures !s.ok ==> !r.ok;
     {
         match c {
@@ -215,29 +254,20 @@ module rv_vale {
             case Function(_, b) => {
                 lemma_FailurePreservedByBlock(b, s, r);
             }
-            case While(c, b) => {
-                var n :| eval_while(c, b, n, s, r);
-            }
-            case IfElse(cond, ifT, ifF) => {
-                var r' :| eval_if_else(cond, ifT, ifF, s, r');
-            }
-            case Ins32(i) => {
-                var r' :| eval_code(c, s, r');
-            }
-            case Comment(com) => {
-                var r' :| eval_code(c, s, r');
+            case _ => {
+                var r' :| r' == s.eval_code(c);
             }
         }
     }
 
-    lemma block_state_validity(block:codes, s:state, r:state)
-        requires eval_block(block, s, r);
+    lemma block_state_validity(block: codes, s: state, r: state)
+        requires r == s.eval_block(block);
         requires valid_state(s);
         decreases block, 0;
         ensures r.ok ==> valid_state(r);
     {
         if block.va_CCons? {
-            var r':state :| eval_code(block.hd, s, r') && eval_block(block.tl, r', r);
+            var r':state :| r' == s.eval_code(block.hd) && r == r'.eval_block(block.tl);
             code_state_validity(block.hd, s, r');
             if r'.ok {
                 block_state_validity(block.tl, r', r);
@@ -248,12 +278,12 @@ module rv_vale {
     }
 
     lemma eval_while_validity(w:cond, c:code, n:nat, s:state, r:state)
-        requires eval_while(w, c, n, s, r);
+        requires r == s.eval_while(c, n);
         decreases c, 1, n;
         ensures valid_state(s) && r.ok ==> valid_state(r);
     {
         if valid_state(s) && r.ok && n > 0 {
-            var r' :| eval_code(c, s, r') && eval_while(w, c, n - 1, r', r);
+            var r' :| r' == s.eval_code(c) && r == r'.eval_while(c, n - 1);
             code_state_validity(c, s, r');
             eval_while_validity(w, c, n - 1, r', r);
             assert valid_state(r);
@@ -261,7 +291,7 @@ module rv_vale {
     }
 
     lemma code_state_validity(c:code, s:state, r:state)
-        requires eval_code(c, s, r);
+        requires r == s.eval_code(c);
         requires valid_state(s);
         decreases c, 0;
         ensures  r.ok ==> valid_state(r);
@@ -271,8 +301,14 @@ module rv_vale {
                 assert true;
             } else if c.Block? {
                 block_state_validity(c.block, s, r);
+            } else if c.IfElse? {
+                if s.eval_cmp(c.cond) {
+                    code_state_validity(c.ifTrue, s, r);
+                } else {
+                    code_state_validity(c.ifFalse, s, r);
+                }
             } else if c.While? {
-                var n:nat :| eval_while(c.whileCond, c.whileBody, n, s, r);
+                var n:nat :| r == s.eval_while(c.whileBody, n);
                 eval_while_validity(c.whileCond, c.whileBody, n, s, r);
                 assert valid_state(r);
             } else if c.Comment? {
@@ -280,7 +316,7 @@ module rv_vale {
         } 
     }
 
-    lemma va_lemma_empty(s: va_state, r: va_state) returns(r': va_state)
+    lemma va_lemma_empty(s: va_state, r: va_state) returns (r': va_state)
         requires eval_code_lax(Block(va_CNil()), s, r)
         ensures  s.ok ==> r.ok
         ensures  r' == s
@@ -290,36 +326,35 @@ module rv_vale {
         r' := s;
     }
 
-    predicate {:opaque} valid_state_opaque(s:state)
-        ensures valid_state_opaque(s) ==> valid_state(s);
-    {
-        valid_state(s)
-    }
+    lemma va_lemma_block(
+        complete_block: codes,
+        s0: va_state,
+        r: va_state)
+    returns(r1: va_state, current:code, rest:codes)
 
-    lemma va_lemma_block(b:codes, s0: va_state, r: va_state) returns(r1: va_state, c0:code, b1:codes)
-        requires b.va_CCons?
-        requires eval_code_lax(Block(b), s0, r)
-        ensures  b == va_CCons(c0, b1)
-        ensures eval_code_lax(c0, s0, r1)
-        ensures c0.Function? ==>
-            eval_code_lax(Block(c0.functionBody), s0, r1);
-        ensures valid_state_opaque(s0) && r1.ok ==> valid_state_opaque(r1);
-        ensures eval_code_lax(Block(b1), r1, r)
+        requires complete_block.va_CCons?
+        requires eval_code_lax(Block(complete_block), s0, r)
+
+        ensures complete_block == va_CCons(current, rest)
+        ensures eval_code_lax(current, s0, r1)
+        ensures current.Function? ==>
+            eval_code_lax(Block(current.functionBody), s0, r1)
+        ensures eval_code_lax(Block(rest), r1, r)
     {
         reveal_eval_code_opaque();
-        c0 := b.hd;
-        b1 := b.tl;
+        current := complete_block.hd;
+        rest := complete_block.tl;
         if s0.ok {
-            assert eval_block(b, s0, r);
-            var r':state :| eval_code(b.hd, s0, r') && eval_block(b.tl, r', r);
-            c0 := b.hd;
-            b1 := b.tl;
-            r1 := state(r'.regs, r'.mem, r'.ok);
+            assert r == s0.eval_block(complete_block);
+            var r':state :| r' == s0.eval_code(complete_block.hd) && r == r'.eval_block(complete_block.tl);
+            current := complete_block.hd;
+            rest := complete_block.tl;
+            r1 := r';
             if valid_state_opaque(s0) {
                 reveal_valid_state_opaque();
-                code_state_validity(c0, s0, r1);
+                code_state_validity(current, s0, r1);
             }
-            assert eval_code_lax(c0, s0, r1);
+            assert eval_code_lax(current, s0, r1);
         } else {
             // If s0 isn't okay, we can do whatever we want,
             // so we ensure r1.ok is false, and hence eval_code_lax(*, r1, *) is trivially true
@@ -327,38 +362,12 @@ module rv_vale {
         }
     }
 
-    lemma va_lemma_ifElse(ifb:cond, ct:code, cf:code, s:va_state, r:va_state) returns(cond:bool, s':va_state)
-        requires valid_state_opaque(s);
-        requires eval_code_lax(IfElse(ifb, ct, cf), s, r)
-        ensures  if s.ok then
-                    && s'.ok
-                    && valid_state_opaque(s')
-                    && cond == eval_cond(s, ifb) 
-                    && s' == s
-                    && (if cond then eval_code_lax(ct, s', r) else eval_code_lax(cf, s', r))
-                else
-                    true
+    predicate {:opaque} eval_while_opaque(w: cond, c: code, n: nat, s: state, r: state)
     {
-        reveal_eval_code_opaque();
-        reveal_valid_state_opaque();
-        cond := eval_cond(s, ifb);
-        if s.ok {
-            assert eval_code(IfElse(ifb, ct, cf), s, r);
-            if cond {
-                code_state_validity(ct, s, r);
-            } else {
-                code_state_validity(cf, s, r);
-            }
-        }
-        s' := s;
+        r == s.eval_while(c, n)
     }
 
-    predicate {:opaque} eval_while_opaque(w:cond, c:code, n:nat, s:state, r:state)
-    {
-        eval_while(w, c, n, s, r)
-    }
-
-    predicate eval_while_lax(w:cond, c:code, n:nat, s:state, r:state)
+    predicate eval_while_lax(w: cond, c: code, n: nat, s: state, r: state)
     {
         s.ok ==> eval_while_opaque(w, c, n, s, r)
     }
@@ -368,27 +377,27 @@ module rv_vale {
         n >= 0 && valid_state_opaque(r1) && eval_while_lax(w, c, n, r1, r2)
     }
 
-    lemma va_lemma_while(w:cond, c:code, s: va_state, r: va_state) returns(n:nat, r': va_state)
+    lemma va_lemma_while(w: cond, c: code, s: va_state, r: va_state) returns(n: nat, r': va_state)
         requires valid_state_opaque(s);
         requires eval_code_lax(While(w, c), s, r)
         ensures  eval_while_lax(w, c, n, r', r)
-        ensures  valid_state_opaque(r');
+        ensures s.ok ==> (n == s.eval_cond(w));
+        ensures valid_state_opaque(r');
         ensures r' == s
-        //ensures  forall c', t, t' :: eval_code(c', t, t') == (t.ok ==> eval_code(c', t, t'));
     {
         reveal_eval_code_opaque();
         reveal_valid_state_opaque();
         reveal_eval_while_opaque();
         if s.ok {
-            assert eval_code(While(w, c), s, r);
-            n :| eval_while(w, c, n, s, r);
+            assert r == s.eval_code(While(w, c));
+            n := s.eval_cond(w);
         } else {
             n := 0;
         }
         r' := s;
     }
 
-    lemma va_lemma_whileTrue(w:cond, c:code, n:nat, s: va_state, r: va_state) returns(s': va_state, r': va_state)
+    lemma va_lemma_whileTrue(w: cond, c: code, n: nat, s: va_state, r: va_state) returns(s': va_state, r': va_state)
         requires n > 0
         requires eval_while_lax(w, c, n, s, r)
         ensures  valid_state_opaque(s) ==> valid_state_opaque(s');
@@ -397,7 +406,6 @@ module rv_vale {
         ensures  if s.ok && valid_state_opaque(s) then
                     && s'.ok
                     && s == s'
-                    && eval_cond(s, w)
                 else
                     true; //!r.ok;
     {
@@ -410,10 +418,10 @@ module rv_vale {
             r' := s;
             return;
         }
-        assert eval_while(w, c, n, s, r); // TODO: Dafny reveal/opaque issue
+        assert r == s.eval_while(c, n); 
 
         if valid_state_opaque(s) {
-            var r'':state :| eval_code(c, s, r'') && eval_while(w, c, n - 1, r'', r);
+            var r'':state :| r'' == s.eval_code(c) && r == r''.eval_while(c, n - 1);
             s' := s;
             r' := r'';
             code_state_validity(c, s', r'');
@@ -423,13 +431,12 @@ module rv_vale {
         }
     }
 
-    lemma va_lemma_whileFalse(w:cond, c:code, s: va_state, r: va_state) returns(r': va_state)
+    lemma va_lemma_whileFalse(w: cond, c: code, s: va_state, r: va_state) returns (r': va_state)
         requires eval_while_lax(w, c, 0, s, r)
         ensures  if s.ok then
                     (if valid_state_opaque(s) then
                         (r'.ok ==> valid_state_opaque(r'))
                     && s == r
-                    && !eval_cond(s, w)
                     && r.ok
                     else
                         true)
@@ -446,5 +453,31 @@ module rv_vale {
             return;
         }
         r' := r;
+    }
+
+    lemma va_lemma_ifElse(ifb: cond, ct:code, cf:code, s:va_state, r:va_state) returns(cond:bool, s':va_state)
+    requires valid_state_opaque(s);
+    requires eval_code_lax(IfElse(ifb, ct, cf), s, r)
+    ensures  if s.ok then
+                && s'.ok
+                && valid_state_opaque(s')
+                && cond == s.eval_cmp(ifb) 
+                && s' == s
+                && (if cond then eval_code_lax(ct, s', r) else eval_code_lax(cf, s', r))
+            else
+                true
+    {
+        reveal_eval_code_opaque();
+        reveal_valid_state_opaque();
+        cond := s.eval_cmp(ifb);
+        if s.ok {
+            assert r == s.eval_code(IfElse(ifb, ct, cf));
+            if cond {
+                code_state_validity(ct, s, r);
+            } else {
+                code_state_validity(cf, s, r);
+            }
+        }
+        s' := s;
     }
 }
